src/spec/TLS13.Record.Spec.fst
@@ -2,6 +2,7 @@ module TLS13.Record.Spec
 
 module B = TLS13.Bytes
 module C = TLS13.Crypto.Spec
+module Seq = FStar.Seq
 module T = TLS13.Types
 
 include TLS13.Messages
@@ -57,3 +58,75 @@ let open_record
        | None -> None)
     else None
   | _, _ -> None
+
+let lemma_open_record_after_seal
+  (st:direction_state)
+  (aad:B.bytes)
+  (pt:plaintext)
+  : Lemma
+      (requires Some? st.key /\ Some? st.static_iv)
+      (ensures (
+        match seal st aad pt with
+        | Some (ct, st') -> open_record st aad ct == Some (pt.fragment, st')
+        | None -> False))
+=
+  match st.key, st.static_iv with
+  | Some key, Some iv ->
+    let nonce = C.tls13_record_nonce iv st.seq in
+    let ct = C.chacha20_poly1305_seal key nonce aad pt.fragment in
+    C.lemma_chacha20_poly1305_open_seal key nonce aad pt.fragment;
+    assert (B.length ct == B.length pt.fragment + 16);
+    assert (B.length ct >= 16)
+  | _, _ ->
+    assert False
+
+let lemma_open_record_after_seal_peer
+  (write_st:direction_state)
+  (read_st:direction_state)
+  (aad:B.bytes)
+  (pt:plaintext)
+  : Lemma
+      (requires
+        write_st.seq == read_st.seq /\
+        (match
+          write_st.key,
+          write_st.static_iv,
+          read_st.key,
+          read_st.static_iv
+        with
+        | Some write_key, Some write_iv, Some read_key, Some read_iv ->
+          Seq.equal write_key read_key /\
+          Seq.equal write_iv read_iv
+        | _, _, _, _ ->
+          False))
+      (ensures (
+        match seal write_st aad pt with
+        | Some (ct, _) -> open_record read_st aad ct == Some (pt.fragment, next_seq read_st)
+        | None -> False))
+=
+  match
+    write_st.key,
+    write_st.static_iv,
+    read_st.key,
+    read_st.static_iv
+  with
+  | Some write_key, Some write_iv, Some read_key, Some read_iv ->
+    Seq.lemma_eq_elim write_key read_key;
+    Seq.lemma_eq_elim write_iv read_iv;
+    assert (C.tls13_record_nonce write_iv write_st.seq ==
+            C.tls13_record_nonce read_iv read_st.seq);
+    C.lemma_chacha20_poly1305_open_seal
+      write_key
+      (C.tls13_record_nonce write_iv write_st.seq)
+      aad
+      pt.fragment;
+    let ct =
+      C.chacha20_poly1305_seal
+        write_key
+        (C.tls13_record_nonce write_iv write_st.seq)
+        aad
+        pt.fragment in
+    assert (B.length ct == B.length pt.fragment + 16);
+    assert (B.length ct >= 16)
+  | _, _, _, _ ->
+    assert False
